main/ts/solutions/lean/LF/Typeclasses.lean
@@ -1712,4 +1712,4 @@ example {α : Type} (x : α) [BEq α] [LawfulBEq α] (xs : List α)
 
 end Reflection
 
--- Source revision: 1a547d1, committed 2026-09-18 21:25 UTC
+-- Source revision: dcf4433, committed 2026-09-24 17:39 UTC
